Trying some semax rules.

progs/verif_threaded_counter.v
@@ -63,6 +63,10 @@ Definition counter_funspecs : funspecs :=
 
 Definition tlock := Tstruct _lock_t noattr.
 Axiom lock_inv : share -> val -> mpred -> mpred.
+
+Axiom lock_inv_share_join : forall sh1 sh2 sh v R, sepalg.join sh1 sh2 sh ->
+  lock_inv sh1 v R * lock_inv sh2 v R = lock_inv sh v R.
+
 Parameter Rlock_placeholder : mpred.
 Parameter spawned_precondition_placeholder : val -> mpred.
 Definition voidstar_funtype :=
@@ -108,25 +112,52 @@ Definition release_spec :=
      LOCAL ()
      SEP (`(lock_inv sh v Rlock_placeholder)).
 
-Definition spawn_thread_spec := (* universe inconsistency if "WITH P" *)
+Parameter spawn_gvars : list (environ -> Prop).
+
+Definition spawn_thread_spec  := (* universe inconsistency if "WITH P" *)
   DECLARE _spawn_thread
    WITH f : val, b : val
-   PRE [_thread_func OF tptr voidstar_funtype, _thread_mutex OF tptr tvoid]
+   PRE [_thread_func OF tptr voidstar_funtype, _thread_mutex_ptr OF tptr tvoid]
      PROP ()
-     LOCAL (temp _thread_mutex b)
+     (LOCALx (temp _thread_mutex_ptr b::spawn_gvars)
      SEP ((EX _y : ident,
      `(func_ptr'
        (WITH y : val
         PRE [ _y OF tptr tvoid ]
           PROP  ()
-          LOCAL (temp _y y)
-          SEP   (`(spawned_precondition_placeholder y))
+          (LOCALx (temp _y y::spawn_gvars)
+          SEP   (`(spawned_precondition_placeholder y)))
         POST [tvoid]
           PROP  ()
           LOCAL ()
           SEP   (emp)
        )
-       f)) ; `(spawned_precondition_placeholder b))
+       f)) ; `(spawned_precondition_placeholder b)))
+   POST [ tvoid ]
+     PROP  ()
+     LOCAL ()
+     SEP   (emp).
+
+Definition funspec_type f_spec :=
+  match f_spec with mk_funspec _ A P Q => A end.
+
+Definition funspec_pre f_spec: funspec_type f_spec -> environ -> mpred :=
+  match f_spec with mk_funspec _ A P Q => P end.
+
+Definition funspec_post f_spec: funspec_type f_spec -> environ -> mpred:=
+  match f_spec with mk_funspec _ A P Q => Q end.
+
+
+Parameter spawned_function_funspec : funspec.
+Definition spawned_function_arg_type: Type := funspec_type spawned_function_funspec.
+
+Definition spawn_thread_spec' := (* universe inconsistency if "WITH P" *)
+  DECLARE _spawn_thread
+   WITH f : val, args_ : spawned_function_arg_type
+   PRE [_thread_func OF tptr voidstar_funtype, _thread_mutex_ptr OF tptr tvoid]
+     PROP ()
+     LOCAL ()
+     SEP (`(func_ptr' spawned_function_funspec f) ; (funspec_pre spawned_function_funspec args_))
    POST [ tvoid ]
      PROP  ()
      LOCAL ()
@@ -160,71 +191,392 @@ Definition thread_invariant v:=
 
 Definition thread_func_spec :=
   DECLARE _thread_func
-   WITH  addof_ctr_lock: val, addof_ctr: val,v : val, sh : share, arg_:val
+  WITH  addof_ctr_lock: val, addof_ctr: val, arg_:val, sh : share
    PRE [_arg OF tptr tvoid]
-     PROP (readable_share sh) (*Holds partial ownerchip of two locks*)
+     PROP () (*Holds partial ownerchip of two locks*)
      LOCAL (temp _arg arg_; gvar _ctr addof_ctr; gvar _ctr_lock addof_ctr_lock)
-     SEP (`(lock_inv sh addof_ctr_lock Rlock_placeholder); `(lock_inv sh arg_ Rlock_placeholder))
+     SEP (`(lock_inv sh addof_ctr_lock Rlock_placeholder); `(lock_inv sh arg_ Rlock_placeholder);
+         `(!!readable_share sh))
    POST [ tvoid ]
      PROP ()
      LOCAL ()
      SEP (`(lock_inv sh arg_ Rlock_placeholder)).
 
-Definition main_spec' :=
+Definition main_spec :=
  DECLARE _main
-  WITH z0: int, addof_ctr: val, ctr: val
+  WITH z0: int, addof_ctr: val, addof_ctr_lock: val, ctr: val
   PRE  [] 
         PROP ()
-        LOCAL(gvar _ctr addof_ctr)
-        SEP( `(data_at Ews tint (repinj tint z0) ctr);`(data_at Ews (tptr tint) ctr addof_ctr))
+        LOCAL(gvar _ctr addof_ctr; gvar _ctr_lock addof_ctr_lock)
+        SEP( `(data_at Ews tint (repinj tint z0) ctr);`(data_at Ews (tptr tint) ctr addof_ctr);
+           `(data_at_ Tsh tlock addof_ctr_lock))
   POST [tint]
   EX z1:int,
         PROP()
         LOCAL( temp ret_temp (Vint (Int.repr 2)))
         SEP( `(data_at Ews tint (repinj tint z1) ctr);`(data_at Ews (tptr tint) ctr addof_ctr)).
 
-Definition main_spec :=
+Definition main_spec' :=
  DECLARE _main
   WITH u : unit
   PRE  [] main_pre prog u
   POST [ tint ] main_post prog u.
 
+(* Malloc *)
+
+Definition natural_alignment := 8.
+
+Definition malloc_compatible (n: Z) (p: val) : Prop :=
+  match p with
+  | Vptr b ofs => (natural_alignment | Int.unsigned ofs) /\
+                           Int.unsigned ofs + n < Int.modulus
+  | _ => False
+  end.
+Definition malloc_spec :=
+ DECLARE _malloc
+  WITH n: Z
+  PRE [ 1%positive OF tuint]
+     PROP (4 <= n <= Int.max_unsigned) 
+     LOCAL (temp 1%positive (Vint (Int.repr n)))
+     SEP ()
+  POST [ tptr tvoid ] 
+     EX v: val,
+     PROP (malloc_compatible n v) 
+     LOCAL (temp ret_temp v) 
+     SEP (`(memory_block Tsh n v)).
 
 Definition Vprog : varspecs := (_ctr_lock, tlock)::(_ctr, tptr tint)::(_zero,tint)::nil.
 
 Definition Gprog : funspecs :=
-  counter_funspecs ++ threads_funspecs ++ concurrent_incr_spec:: thread_func_spec::main_spec::nil.
+  counter_funspecs ++ threads_funspecs ++ concurrent_incr_spec::
+                   malloc_spec :: thread_func_spec::main_spec::nil.
 
 
 (*Lets do this first:*)
 
+Definition counter_invariant addof_ctr:=
+  EX z : Z, EX ctr : val, 
+   (data_at Ews tint (repinj tint (Int.repr z)) ctr)*(data_at Ews (tptr tint) ctr addof_ctr).
+
 Lemma body_main:  semax_body Vprog Gprog f_main main_spec.
 Proof.
   start_function.
-  normalize; intros zero_.
-  normalize; intros addof_ctr.
-  normalize; intros ctr_lock_.
-  normalize; simpl.
-  normalize; simpl.
-
-  apply something.
-  normalize; simpl.
+  
+  (*call reset*)
   forward_call  (z0 , addof_ctr, ctr).
+
+  (*call makelock(&ctr_lock)*)
+  pose (sh := Share.top).
+  assert (Wsh: writable_share sh) by apply semax_call.writable_share_top.
+  normalize.
+  forward_call (addof_ctr_lock , sh).
+
+  (*call release(&ctr_lock)*)
+  assert (RLock_ctr: Rlock_placeholder = (counter_invariant addof_ctr)) by admit.
+  forward_call (addof_ctr_lock , sh).
+  rewrite RLock_ctr.
+  unfold counter_invariant.
+  normalize. apply exp_right with (0).
+  normalize. apply exp_right with ctr.
+  fold Int.zero. cancel.
+
+  (*call malloc(thread_mutex_ptr)*)
+  (* rewrite <- seq_assoc. *)
+  normalize.
+  forward_call 24%Z _thread_mutex_ptr.
+  solve [compute; intuition; congruence].
   
+  (*call makelock(&thread_mutex)*)
+  normalize.
+  forward_call (_thread_mutex_ptr , sh).
+  rewrite <- memory_block_data_at_; simpl.
+  cancel.
+   (* Proof field_compatible tlock [] _thread_mutex_ptr*) 
+  {
+  unfold malloc_compatible in H; destruct _thread_mutex_ptr; try solve[inversion H].
+  unfold field_compatible; intuition.
+  - unfold isptr; auto.
+  - compute; reflexivity.
+  - simpl. omega.
+  - simpl. unfold align_attr, attr_alignas, noattr.
+    eapply (Zdivides_trans _ 8 _). exists 2; omega. exact H0.
+  - simpl; trivial.
+  }
+
+  (*call spawn*)
+
+Lemma semax_fun_id'' id f Espec {cs} Delta P Q R Post c :
+  (var_types Delta) ! id = None ->
+  (glob_specs Delta) ! id = Some f ->
+  (glob_types Delta) ! id = Some (type_of_funspec f) ->
+  @semax cs Espec Delta
+    (EX v : val, PROPx P
+      (LOCALx (gvar id v :: Q)
+      (SEPx (`(func_ptr' f v) :: R)))) c Post ->
+  @semax cs Espec Delta (PROPx P (LOCALx Q (SEPx R))) c Post.
+Proof.
+intros V G GS SA.
+apply (semax_fun_id id f Delta); auto.
+eapply semax_pre_post; try apply SA; [ clear SA | intros; entailer ].
+go_lowerx.
+apply exp_right with (eval_var id (type_of_funspec f) rho).
+entailer.
+apply andp_right.
+- (* about gvar *)
+  apply prop_right.
+  unfold gvar, eval_var, Map.get.
+  destruct H as (_ & _ & DG & DS).
+  destruct (DS id _ GS) as [-> | (t & E)]; [ | congruence].
+  destruct (DG id _ GS) as (? & -> & ?); auto.
+
+- (* about func_ptr/func_ptr' *)
+  unfold func_ptr'.
+  rewrite <- andp_left_corable, andp_comm; auto.
+  apply corable_func_ptr.
+Qed.
+
+
+Lemma split_readable_share sh :
+  readable_share sh ->
+  exists sh1, exists sh2,
+    readable_share sh1 /\
+    readable_share sh2 /\
+    sepalg.join sh1 sh2 sh.
+Admitted.
+
+Lemma split_Tsh :
+  exists sh1, exists sh2,
+    readable_share sh1 /\
+    readable_share sh2 /\
+    sepalg.join sh1 sh2 Tsh.
+Proof.
+  apply split_readable_share; auto.
+Qed.
+
+
+Ltac get_global_function'' _f :=
+  eapply (semax_fun_id'' _f); try reflexivity.
   
+  get_global_function'' _thread_func.
+  normalize.
+  apply extract_exists_pre; intros thread_func_.
+
+
+
+
+
+
+
+
+
+
+
+(*
+  
+  (*SEMAX RULE for spawn*)
+  Definition spawn_expr name:=
+    (Evar name  (* Name is an identifier, that in the future will be fixed. *)
+          (Tfunction (* It's a function, under the hood *)
+             (Tcons (tptr (Tfunction (Tcons (tptr tvoid) Tnil)  (tptr tvoid) cc_default)) (Tcons (tptr tvoid) Tnil)) tvoid cc_default)).
+  
+  Definition Sspawn' name f arg:=
+    Scall                      (* Clighen comiles spawn as a function. *)
+      None                     (* Spawning doesn't return anything. *)
+      (spawn_expr name)        (* The typed expression of spawn as a function*)
+      [f; arg]  (* One single argument of type (void * ) *)
+  .
+
+
+
+
+
+
+
+  
+  (*Have to do this in every file using the rule, until the function gets a fixed name. *)
+  Definition Sspawn:= Sspawn' _spawn_thread.
+  
+Axiom semax_spawn : 
+  forall {Espec: OracleKind}{CS: compspecs},
+  forall Delta A (P Q: A -> environ -> mpred) (x: A) (F: environ -> mpred)
+          arg_name a b,
+           Cop.classify_fun (typeof a) =
+           Cop.fun_case_f (type_of_params [(arg_name , tptr tvoid)]) tvoid cc_default ->
+          tc_fn_return Delta None tvoid ->
+  @semax CS Espec Delta
+          ((tc_expr Delta a) && (tc_expr Delta b)  && 
+         (`(func_ptr (mk_funspec  ([(arg_name , tptr tvoid)],tvoid) A P Q)) (eval_expr a) &&   
+          (F * `(P x) (make_args' ([(arg_name , tptr tvoid)],tvoid) (fun env=> [eval_expr b env])))))
+         (Sspawn a b)
+         (normal_ret_assert  
+            ( F )).
+
+
+eapply semax_seq'.
+unfold PROPx, LOCALx, SEPx; simpl.
+normalize.
+rewrite local_lift2_and.
+assert ().
+rewrite andp_unfold.
+repeat rewrite <- andp_assoc.
+unfold fold_right.
+repeat rewrite local_lift2_and.
+unfold func_ptr'.
+rewrite local_unfold.
+repeat rewrite local_unfold.
+lift1.
+eapply semax_spawn.
+
+
+  
+  (* build the spawned frame *)
+  
+Axiom semax_spawn : 
+  forall {Espec: OracleKind}{CS: compspecs},
+    forall Delta A (P Q: A -> environ -> mpred) (x: A) (F: environ -> mpred) ret argsig retsig a bl,
+           Cop.classify_fun (typeof a) =
+           Cop.fun_case_f (type_of_params argsig) retsig cc_default ->
+           (retsig = Tvoid -> ret = None) ->
+          tc_fn_return Delta ret retsig ->
+  @semax CS Espec Delta
+          ((tc_expr Delta a) && (tc_exprlist Delta (snd (split argsig)) bl)  && 
+         (`(func_ptr (mk_funspec  (argsig,retsig) A P Q)) (eval_expr a) &&   
+          (F * `(P x) (make_args' (argsig,retsig) (eval_exprlist (snd (split argsig)) bl)))))
+         (Scall ret a bl)
+         (normal_ret_assert  
+          (EX old:val, substopt ret (`old) F * maybe_retval (Q x) retsig ret)).
+*)
+
+
+  
+  destruct split_Tsh as (sh1 & sh2 & Rsh1 & Rsh2 & Join).
+  rewrite <- (lock_inv_share_join _ _ _ _ _ Join).
+  
+  pose (spawned_precondition := 
+    fun (addof_ctr_lock: val) (addof_ctr: val)(v : val)( sh : share)( arg_:val) =>
+    `(lock_inv sh addof_ctr_lock Rlock_placeholder) *
+                   `(lock_inv sh arg_ Rlock_placeholder)).
+  normalize.
+
+assert (__AXIOM1__: spawned_function_funspec =  snd thread_func_spec) by admit.
+assert (__AXIOM2__: spawn_gvars =  [gvar _ctr addof_ctr; gvar _ctr_lock addof_ctr_lock]) by admit.
+
+  pose (witness:= (thread_func_, (addof_ctr_lock,  addof_ctr, _thread_mutex_ptr,sh ))).
+  eapply semax_seq'.
+
+let Frame := fresh "Frame" in
+evar (Frame: list (mpred)).
+
+
+
+{ eapply (semax_call_id00_wow witness Frame).
+  - reflexivity.
+  - simpl. f_equal.
+    unfold spawned_function_arg_type. rewrite __AXIOM__.
+    unfold thread_func_spec; simpl.
+    f_equal; reflexivity.
+  - reflexivity.
+  - reflexivity.
+  - prove_local2ptree.
+  - repeat constructor.
+  - entailer.
+  - reflexivity.
+  - prove_local2ptree.
+  - repeat constructor.
+    unfold PROPx, LOCALx, SEPx; simpl.
+    unfold local, lift1.
+    econstructor.
+    simpl.
+    
+    entailer.
+  - reflexivity.
+
+    
+try reflexivity.
+reflexivity.
+
+ [ reflexivity | reflexivity | reflexivity | reflexivity
+ | prove_local2ptree | repeat constructor 
+ | try apply local_True_right; entailer!
+ | reflexivity
+ | prove_local2ptree | repeat constructor 
+ | reflexivity | reflexivity
+ | Forall_pTree_from_elements
+ | Forall_pTree_from_elements
+ | unfold fold_right at 1 2; cancel
+ | cbv beta iota; 
+    repeat rewrite exp_uncurry;
+    try rewrite no_post_exists0; 
+    first [reflexivity | extensionality; simpl; reflexivity]
+ | intros; try match goal with  |- extract_trivial_liftx ?A _ =>
+        (has_evar A; fail 1) || (repeat constructor)
+     end
+ | unify_postcondition_exps
+ | unfold fold_right_and; repeat rewrite and_True; auto
+ ].
+
+Ltac simpl_strong_cast :=
+try match goal with |- context [strong_cast ?t1 ?t2 ?v] =>
+  first [change (strong_cast t1 t2 v) with v
+         | change (strong_cast t1 t2 v) with
+                (force_val (sem_cast t1 t2 v))
+          ]
+end.
+
+  
+  forward_call_id00_wow (thread_func_, _thread_mutex_ptr).
+          | after_forward_call ]
   
   eapply semax_seq'.
-  forward_call_id00_wow (z0 , addof_ctr, ctr).
-     [first [forward_call_id1_wow witness
+             forward_call_id1_wow witness.
            | forward_call_id1_x_wow witness
            | forward_call_id1_y_wow witness
            | forward_call_id01_wow witness ]
      | after_forward_call
      ]
-  fwd_call' (z0 , addof_ctr, ctr).
-  forward_call (z0 , addof_ctr, ctr).
+  |  eapply semax_seq'; [forward_call_id00_wow witness 
+          | after_forward_call ]
+  | rewrite <- seq_assoc; fwd_call' witness
+  ].
 
 
+  
+  
+  fwd_call' (thread_func_, _thread_mutex_ptr).
+  forward_call (thread_func_, _thread_mutex_ptr).
+
+
+Definition spawn_thread_spec := (* universe inconsistency if "WITH P" *)
+  DECLARE _spawn_thread
+   WITH f : val, _thread_mutex_ptr : val
+   PRE [_thread_func OF tptr voidstar_funtype, Top._thread_mutex_ptr OF tptr tvoid]
+     PROP ()
+     LOCAL (temp Top._thread_mutex_ptr _thread_mutex_ptr)
+     SEP ((EX _y : ident,
+     `(func_ptr'
+       (WITH y : val * val * share * val
+        PRE [ _y OF tptr tvoid ]
+          (let (p, arg_) := x in
+            let (p0, sh0) := p in
+            let (addof_ctr_lock0, addof_ctr0) := p0 in
+          PROP  ()
+          LOCAL (temp _arg y)
+          SEP   (`(spawned_precondition_placeholder y)))
+        POST [tvoid]
+          PROP  ()
+          LOCAL ()
+          SEP   (emp)
+       )
+       f)) ; `(spawned_precondition_placeholder _thread_mutex_ptr))
+   POST [ tvoid ]
+     PROP  ()
+     LOCAL ()
+     SEP   (emp).
+
+
+
+  
+  
 Lemma body_thread_func_spec:semax_body Vprog Gprog f_thread_func thread_func_spec.
 Proof.
   start_function.
@@ -236,11 +588,11 @@ Proof.
   forward_call (addof_ctr_lock, addof_ctr, sh).
 
   (* The invariant can't be set up 'legaly' because of universe inconsistency *)
-  assert (HH: Rlock_placeholder = thread_invariant addof_ctr_lock) by admit.
+  assert (RLock_thr: Rlock_placeholder = thread_invariant addof_ctr_lock) by admit.
 
   (*call release*)
   forward_call (arg_, sh).
-  rewrite HH at 2. unfold thread_invariant.
+  rewrite RLock_thr at 2. unfold thread_invariant.
   normalize. 
   apply exp_right with (sh). cancel.
 
@@ -257,13 +609,10 @@ Lemma body_concurrent_incr:  semax_body Vprog Gprog f_concurrent_incr concurrent
 
   
   (*call incr*)
-  Definition counter_invariant addof_ctr:=
-  EX z : Z, EX ctr : val, 
-  (data_at Ews tint (repinj tint (Int.repr z)) ctr)*(data_at Ews (tptr tint) ctr addof_ctr).
 
   (* The invariant can't be set up 'legaly' because of universe inconsistency *)
-  assert (HH: Rlock_placeholder = (counter_invariant addof_ctr)) by admit.
-  rewrite HH.
+  assert (RLock_ctr: Rlock_placeholder = (counter_invariant addof_ctr)) by admit.
+  rewrite RLock_ctr.
   unfold counter_invariant at 2.
 
   
